
\newpage
\section{Formulas}

\begin{align*}
& \cp_1(c) = y-z, \qquad
\cp_1(y) = \cp_1(z) = 0, \\
& \cp_2(c) = - \frac{1}{2} c (y+x) - \frac{1}{2} (y+x) c, \qquad
\cp_2(y) = - y y, \qquad
\cp_2(z) = - z z, \\
& \cp_3(c) = \frac{1}{12} (y-z) c c + \frac{1}{6} c (y-z) c + \frac{1}{12} c c (y-z), \qquad
\cp_3(y) = \cp_3(z) = 0, \qquad k \geq 3.
\end{align*}
Then
\begin{align*}
\cp_1(cc) &= \cp_1(c)c - c\cp_1(c) \\
\cp_2(cc) &= (1324) \cp_2(c)\cp_2(c) \\
\cp_3(cc) &= (135246) \Big( - (\cp_2 \otimes \id) \cp_2(\c) \otimes \cp_3(\c) + \cp_3(\c) \otimes (\id \otimes \cp_2) \cp_2(c) \Big) \\
\end{align*}

\newpage

\section{Old Formulas}

Let us study the cube with to generator $\c\c$.
Denote $x = y-z$ and $\x = y+z$.
Recall

\begin{align*}
& \cp_1(c) = y-z, \qquad
\cp_1(y) = \cp_1(z) = 0, \\
& \cp_2(c) = -\frac{1}{2} (c \x + \x c), \qquad
\cp_2(y) = -y y, \qquad
\cp_2(z) = -z z, \\
& \cp_3(c) = \frac{1}{12} x c c + \frac{1}{6} c x c + \frac{1}{12} c c x, \qquad
\cp_3(y) = \cp_3(z) = 0, \qquad k \geq 3.
\end{align*}
Then
\begin{align*}
\cp_1(cc) &=
\cp_1(c)c - c\cp_1(c) \\ &=
xc - cx. \\
\cp_2(cc) &=
(1324) \cp_2(c)\cp_2(c) =
\frac{1}{4} (1324) \Big( c \ot \bar{x} + \bar{x} \ot c \Big) \Big\vert \Big( c \ot \bar{x} + \bar{x} \ot c \Big) \\ &=
\frac{1}{4} (\x\x \mid \c\c - \x\c \mid \c\x + \c\x \mid \x\c + \c\c \mid \x\x) \\
\cp_3(cc) &= (135246) \big( - (\cp_2 \otimes \id) \cp_2(\c) \otimes \cp_3(\c) + \cp_3(\c) \otimes (\id \otimes \cp_2) \cp_2(c) \big) \\
&= (135246) \Big( \frac{1}{2} (\cp_2 \otimes \id) (\c\x + \x\c) \otimes \big( \frac{1}{12} x c c + \frac{1}{6} c x c + \frac{1}{12} c c x \big) \\ & \quad +
\big( \frac{1}{12} x c c + \frac{1}{6} c x c + \frac{1}{12} c c x \big) \otimes - \frac{1}{2} (\id \otimes \cp_2) (c \x + \x c ) \Big) \\
&= (135246) \Big( -\frac{1}{4} (\c\x\x + \x\c\x + 2\x\x\c) \otimes \big( \frac{1}{12} x c c + \frac{1}{6} c x c + \frac{1}{12} c c x \big) \\ & \quad +
\big( \frac{1}{12} x c c + \frac{1}{6} c x c + \frac{1}{12} c c x \big) \otimes - \frac{1}{2} (\id \otimes \cp_2) (c \x + \x c ) \Big) \\
\end{align*}