\[
\boxed{\Delta_3(c) =
\frac{1}{12} \ (y-z) \ot c \ot c + \frac{1}{6} \ c \ot (y-z) \ot c + \frac{1}{12} \ c \ot c \ot (y-z)}
\]

\noindent $i=3, k=1, n=0$:
\begin{align*}
(-1)^1 \big( \id_C^{\ot 2} \ot \Delta_1 \ot \id_C^{\ot 0} \big) \Delta_3(c) & =
+ \frac{1}{12} \ (y-z) \ot c \ot (y-z) + \frac{1}{6} \ c \ot (y-z) \ot (y-z)
\end{align*}

\noindent $i=3, k=1, n=1$:
\begin{align*}
(-1)^3 \big( \id_C^{\ot 1} \ot \Delta_1 \ot \id_C^{\ot 1} \big) \Delta_3(c) =
- \frac{1}{12} \ (y-z) \ot (y-z) \ot c + \frac{1}{12} \ c \ot (y-z) \ot (y-z)
\end{align*}

\noindent $i=3, k=1, n=2$:
\begin{align*}
(-1)^5 \big( \id_C^{\ot 0} \ot \Delta_1 \ot \id_C^{\ot 2} \big) \Delta_3(c) =
-\frac{1}{6} \ (y-z) \ot (y-z) \ot c - \frac{1}{12} \ (y-z) \ot c \ot (y-z)
\end{align*}

\[
\boxed{\Delta_2(c) = -\frac{1}{2} \Big( c \ot (y+z) + (y+z) \ot c \Big)}
\]

\noindent $i=3, k=2, n=0$:
\begin{align*}
(-1)^2 \big( \id_C^{\ot 1} \ot \Delta_2 \ot \id_C^{\ot 0} \big) \Delta_2(c) &=
- \frac{1}{2} \Big( c \ot \Delta_2(y+z) + (y+z) \ot \Delta_2(c) \Big) \\ &=
+ \frac{1}{2} c \ot y \ot y + \frac{1}{2} c \ot z \ot z +
\frac{1}{4} \ (y+z) \ot c \ot (y+z) + \frac{1}{4} \ (y+z) \ot (y+z) \ot c
\end{align*}

\noindent $i=3, k=2, n=1$:
\begin{align*}
(-1)^5 \big( \id_C^{\ot 0} \ot \Delta_2 \ot \id_C^{\ot 1} \big) \Delta_2(c) &=
+ \frac{1}{2} \Big( \Delta_2(c) \ot (y+z) + \Delta_2(y+z) \ot c \Big) \\ &=
- \frac{1}{4} \ c \ot (y+z) \ot (y+z) - \frac{1}{4} \ (y+z) \ot c \ot (y+z)
- \frac{1}{2} y \ot y \ot c - \frac{1}{2} z \ot z \ot c
\end{align*}

\noindent $i=3, k=3, n=0$:
\begin{align*}
(-1)^3 \big( \id_C^{\ot 0} \ot \Delta_3 \ot \id_C^{\ot 0} \big) \Delta_1(c) = 0
\end{align*}

There are two pairs of summands that cancel immediately and two pairs that can be combined.
After multiplying by $12$ we get:
\begin{align*}
3 c \ot (y-z) \ot (y-z) \ - \
3 (y-z) \ot (y-z) \ot c \ + \ \\
3 (y+z) \ot (y+z) \ot c \ - \
3 c \ot (y+z) \ot (y+z) \\
6 c \ot y \ot y \ + \
6 c \ot z \ot z \ - \
6 y \ot y \ot c \ - \
6 z \ot z \ot c
\end{align*}

\anibal{works if the first line has the opposite sign which is implied if $\Delta_3$ does.}
